Stuck with universe polymorphism (HandlerFacts)

theories/Indexed/Sum.v
@@ -1,14 +1,15 @@
 (** Sums of effects *)
 
-Set Implicit Arguments.
-Set Contextual Implicit.
-
 From Coq Require Import
      Lists.List.
 
 From ITree Require Import
      Basics.Basics
      Core.ITree.
+
+Set Implicit Arguments.
+Set Contextual Implicit.
+Set Universe Polymorphism.
 
 (** Sums for extensible event types. *)
 
@@ -25,61 +26,4 @@ Notation "E1 +' E2" := (sum1 E1 E2)
 Notation "EE ++' E" := (List.fold_right sum1 EE E)
   (at level 50, left associativity) : type_scope.
 
-Variant emptyE : Type -> Type := .
-
-Module Sum1.
-
-(* Just for this section, [A B C D : Type -> Type] are more
-   effect types. *)
-
-Definition elim_emptyE {A} : emptyE ~> A :=
-  fun X (e : emptyE X) => match e with end.
-
-Definition idE {A : Type -> Type} : A ~> A :=
-  fun X (e : A X) => e.
-
-Definition cmpE {A B C : Type -> Type} : (B ~> C) -> (A ~> B) -> (A ~> C) :=
-  fun g f X a => g X (f X a).
-
-
-(** [Sum1.swap] *)
-Definition swap {A B : Type -> Type} : A +' B ~> B +' A :=
-  fun _ ab =>
-    match ab with
-    | inl1 a => inr1 a
-    | inr1 b => inl1 b
-    end.
-
-(** [Sum1.bimap] *)
-Definition bimap {A B C D : Type -> Type}
-           (f : A ~> B) (g : C ~> D) : A +' C ~> B +' D :=
-  fun _ ab =>
-    match ab with
-    | inl1 a => inl1 (f _ a)
-    | inr1 b => inr1 (g _ b)
-    end.
-
-Definition elim {A B C : Type -> Type}
-           (f : A ~> C) (g : B ~> C) : A +' B ~> C :=
-  fun _ ab =>
-    match ab with
-    | inl1 a => f _ a
-    | inr1 b => g _ b
-    end.
-
-(** [Sum1.assoc] *)
-Definition assoc {A B C : Type -> Type} : A +' (B  +' C) ~> (A +' B) +' C :=
-  fun _ abc =>
-    match abc with
-    | inl1 a => inl1 (inl1 a)
-    | inr1 (inl1 b) => inl1 (inr1 b)
-    | inr1 (inr1 c) => inr1 c
-    end.
-
-Definition emptyE_left {A : Type -> Type} : emptyE +' A ~> A :=
-  elim elim_emptyE idE.
-
-Definition emptyE_right {A : Type -> Type} : A +' emptyE ~> A :=
-  elim idE elim_emptyE.
-
-End Sum1.
+Variant void1 : Type -> Type := .
