examples/stlc.v
@@ -56,7 +56,7 @@ Fixpoint subst (n : nat) (s t : term) :=
   end.
 
 (* big-step call-by-value *)
-Definition big_step : term -> itree emptyE value :=
+Definition big_step : term -> itree void1 value :=
   rec (fun t =>
     match t with
     | Var n => ret (VHead (VVar n))
