theories/Indexed/OpenSum.v
@@ -56,7 +56,7 @@ Instance Subeffect_right {A B C} `(A -< C) : A -< B +' C | 9 :=
     for the inclusion [E -< E +' E +' F]. *)
 
 (** Initial object of the [Subeffect] category. *)
-Instance Subeffect_empty A : emptyE -< A :=
+Instance Subeffect_empty A : void1 -< A :=
   { subeffect _ v := match v with end }.
 
 (** Notations to construct and pattern-match on nested sums. *)
